coqimp/example/lib/reg_lemma.v
@@ -901,12 +901,13 @@ Proof.
 Qed.
  
 Theorem add_rule_reg :
-  forall grst rs rd p oexp v1 v2,
+  forall grst rs rd p oexp v1 v2 v,
+    Some v = val_add v1 v2 ->
     get_genreg_val grst rs = v1 -> eval_opexp_reg grst oexp = Some v2 ->
     |- {{ GenRegs grst ** p }} add rs oexp rd
-                              {{ GenRegs (upd_genreg grst rd (v1 +ᵢ v2)) ** p }}.
+                              {{ GenRegs (upd_genreg grst rd v) ** p }}.
 Proof.
-  intros.
+  introv Hres; intros.
   eapply ins_conseq_rule.
   eauto.
   eapply add_rule; eauto.
@@ -915,7 +916,6 @@ Proof.
     simpl.
     split.
     {
-      instantiate (1 := v1).
       sep_star_split_tac.
       simpl in H5.
       simpljoin1.
@@ -924,7 +924,6 @@ Proof.
       eapply get_R_merge_still; eauto.
     }
     {
-      instantiate (1 := v2).
       sep_star_split_tac.
       simpl in H5.
       simpljoin1.
@@ -945,12 +944,13 @@ Proof.
 Qed.
 
 Theorem sub_rule_reg :
-  forall grst rs rd p oexp v1 v2,
+  forall grst rs rd p oexp v1 v2 v,
+    Some v = val_sub v1 v2 ->
     get_genreg_val grst rs = v1 -> eval_opexp_reg grst oexp = Some v2 ->
     |- {{ GenRegs grst ** p }} sub rs oexp rd
-                              {{ GenRegs (upd_genreg grst rd (v1 -ᵢ v2)) ** p }}.
+                              {{ GenRegs (upd_genreg grst rd v) ** p }}.
 Proof.
-  intros.
+  introv Hres; intros.
   eapply ins_conseq_rule.
   eauto.
   eapply sub_rule; eauto.
@@ -959,7 +959,6 @@ Proof.
     simpl.
     split.
     {
-      instantiate (1 := v1).
       sep_star_split_tac.
       simpl in H5.
       simpljoin1.
@@ -968,7 +967,6 @@ Proof.
       eapply get_R_merge_still; eauto.
     }
     {
-      instantiate (1 := v2).
       sep_star_split_tac.
       simpl in H5.
       simpljoin1.
@@ -990,9 +988,9 @@ Qed.
 
 Theorem and_rule_reg :
   forall grst rs rd p oexp v1 v2,
-    get_genreg_val grst rs = v1 -> eval_opexp_reg grst oexp = Some v2 ->
+    get_genreg_val grst rs = W v1 -> eval_opexp_reg grst oexp = Some (W v2) ->
     |- {{ GenRegs grst ** p }} and rs oexp rd
-                              {{ GenRegs (upd_genreg grst rd (v1 &ᵢ v2)) ** p }}.
+                              {{ GenRegs (upd_genreg grst rd (W v1 &ᵢ v2)) ** p }}.
 Proof.
   intros.
   eapply ins_conseq_rule.
@@ -1002,7 +1000,7 @@ Proof.
     intros.
     simpl.
     split.
-    {
+    { 
       instantiate (1 := v1).
       sep_star_split_tac.
       simpl in H5.
@@ -1010,6 +1008,7 @@ Proof.
       simpl.
       eapply getR_eq_get_genreg_val in H1; eauto.
       eapply get_R_merge_still; eauto.
+      rewrite H in H1; eauto.
     }
     {
       instantiate (1 := v2).
@@ -1034,9 +1033,9 @@ Qed.
 
 Theorem or_rule_reg :
   forall grst rs rd p oexp v1 v2,
-    get_genreg_val grst rs = v1 -> eval_opexp_reg grst oexp = Some v2 ->
+    get_genreg_val grst rs = W v1 -> eval_opexp_reg grst oexp = Some (W v2) ->
     |- {{ GenRegs grst ** p }} or rs oexp rd
-                              {{ GenRegs (upd_genreg grst rd (v1 |ᵢ v2)) ** p }}.
+                              {{ GenRegs (upd_genreg grst rd (W v1 |ᵢ v2)) ** p }}.
 Proof.
   intros.
   eapply ins_conseq_rule.
@@ -1054,6 +1053,7 @@ Proof.
       simpl.
       eapply getR_eq_get_genreg_val in H1; eauto.
       eapply get_R_merge_still; eauto.
+      rewrite H in H1; eauto.
     }
     {
       instantiate (1 := v2).
@@ -1078,9 +1078,9 @@ Qed.
 
 Theorem sll_rule_reg :
   forall grst rs rd p oexp v1 v2,
-    get_genreg_val grst rs = v1 -> eval_opexp_reg grst oexp = Some v2 ->
+    get_genreg_val grst rs = W v1 -> eval_opexp_reg grst oexp = Some (W v2) ->
     |- {{ GenRegs grst ** p }} sll rs oexp rd
-                              {{ GenRegs (upd_genreg grst rd (v1 <<ᵢ (get_range 0 4 v2))) ** p }}.
+                              {{ GenRegs (upd_genreg grst rd (W v1 <<ᵢ (get_range 0 4 v2))) ** p }}.
 Proof.
   intros.
   eapply ins_conseq_rule.
@@ -1098,6 +1098,7 @@ Proof.
       simpl.
       eapply getR_eq_get_genreg_val in H1; eauto.
       eapply get_R_merge_still; eauto.
+      rewrite H in H1; eauto.
     }
     {
       instantiate (1 := v2).
@@ -1122,9 +1123,9 @@ Qed.
 
 Theorem srl_rule_reg :
   forall grst rs rd p oexp v1 v2,
-    get_genreg_val grst rs = v1 -> eval_opexp_reg grst oexp = Some v2 ->
+    get_genreg_val grst rs = W v1 -> eval_opexp_reg grst oexp = Some (W v2) ->
     |- {{ GenRegs grst ** p }} srl rs oexp rd
-                              {{ GenRegs (upd_genreg grst rd (v1 >>ᵢ (get_range 0 4 v2))) ** p }}.
+                              {{ GenRegs (upd_genreg grst rd (W v1 >>ᵢ (get_range 0 4 v2))) ** p }}.
 Proof.
   intros.
   eapply ins_conseq_rule.
@@ -1142,6 +1143,7 @@ Proof.
       simpl.
       eapply getR_eq_get_genreg_val in H1; eauto.
       eapply get_R_merge_still; eauto.
+      rewrite H in H1; eauto.
     }
     {
       instantiate (1 := v2).
@@ -1189,7 +1191,7 @@ Theorem getcwp_rule_reg :
   forall grst rd p id F,
     |- {{ GenRegs grst ** {| id, F|} ** p }}
         getcwp rd
-        {{ GenRegs (upd_genreg grst rd id) ** {| id, F|} ** p }}.
+        {{ GenRegs (upd_genreg grst rd (W id)) ** {| id, F|} ** p }}.
 Proof.
   intros.
   eapply ins_conseq_rule.
@@ -1214,10 +1216,10 @@ Qed.
 
 Theorem ld_rule_reg :
   forall p aexp rd grst v l,
-    eval_addrexp_reg grst aexp = Some l ->
+    eval_addrexp_reg grst aexp = Some (Ptr l) ->
     |- {{ GenRegs grst ** l |-> v ** p }}
         ld aexp rd
-        {{ GenRegs (upd_genreg grst rd v) ** l |-> v ** p }}.
+       {{ GenRegs (upd_genreg grst rd v) ** l |-> v ** p }}.
 Proof.
   intros.
   eapply ins_conseq_rule.
@@ -1257,7 +1259,7 @@ Qed.
 
 Theorem st_rule_reg :
   forall p aexp rs grst v v' l,
-    eval_addrexp_reg grst aexp = Some l -> get_genreg_val grst rs = v' ->
+    eval_addrexp_reg grst aexp = Some (Ptr l) -> get_genreg_val grst rs = v' ->
     |- {{ GenRegs grst ** l |-> v ** p }}
         st rs aexp
         {{ GenRegs grst ** l |-> v' ** p }}.
@@ -1302,27 +1304,26 @@ Qed.
 
 Theorem save_rule_reg :
   forall p (rs rd : GenReg) (id id' : Word) (F : FrameList)
-    (fm1 fm2 fmg fmo fml fmi : Frame) (v1 v2 v v' : Word) (oexp : OpExp),
+         (fm1 fm2 fmg fmo fml fmi : Frame) (v : Word) v1 v2 res (oexp : OpExp),
+    Some res = val_add v1 v2 ->
     get_genreg_val (fmg, fmo, fml, fmi) rs = v1 ->
     eval_opexp_reg (fmg, fmo, fml, fmi) oexp = Some v2 ->
     id' = pre_cwp id -> win_masked id' v = false ->
-    |- {{ GenRegs (fmg, fmo, fml, fmi) ** Rwim |=> v ** {| id, F ++ [fm1; fm2] |} ** p }}
+    |- {{ GenRegs (fmg, fmo, fml, fmi) ** Rwim |=> W v ** {| id, F ++ [fm1; fm2] |} ** p }}
         save rs oexp rd
-      {{ GenRegs (upd_genreg (fmg, fm1, fm2, fmo) rd (v1 +ᵢ v2)) ** Rwim |=> v **
+      {{ GenRegs (upd_genreg (fmg, fm1, fm2, fmo) rd res) ** Rwim |=> W v **
                  {| id', fml :: fmi :: F |} ** p }}.
 Proof.
-  intros.
+  introv Hres; intros.
   eapply ins_conseq_rule.
-  instantiate (1 := Rwim |=> v ** GenRegs (fmg, fmo, fml, fmi) **
+  instantiate (1 := Rwim |=> W v ** GenRegs (fmg, fmo, fml, fmi) **
                          {|id, F ++ [fm1; fm2]|} ** p).
   intros.
   sep_cancel1 2 1.
   eauto.
-  eapply save_rule.
-  {
+  eapply save_rule; eauto.
+  { 
     intros.
-    instantiate (2 := v1).
-    instantiate (1 := v2).
     sep_star_split_tac.
     simpl in H6, H7.
     simpljoin1.
@@ -1353,12 +1354,6 @@ Proof.
     eapply astar_comm.
     sep_cancel1 1 1.
     eauto.
-  }
-  {
-    eauto.
-  }
-  {
-    eauto.
   } 
   {
     intros.
@@ -1378,18 +1373,19 @@ Qed.
 
 Theorem restore_rule_reg :
   forall p (rs rd : GenReg) (id id' : Word) (F : FrameList)
-    (fm1 fm2 fmg fmo fml fmi : Frame) (v1 v2 v v' : Word) (oexp : OpExp),
+         (fm1 fm2 fmg fmo fml fmi : Frame) v1 v2 v (res : Val) (oexp : OpExp),
+    Some res = val_add v1 v2 ->
     get_genreg_val (fmg, fmo, fml, fmi) rs = v1 ->
     eval_opexp_reg (fmg, fmo, fml, fmi) oexp = Some v2 ->
     id' = post_cwp id -> win_masked id' v = false ->
-    |- {{ GenRegs (fmg, fmo, fml, fmi) ** Rwim |=> v ** {| id, fm1 :: fm2 :: F |} ** p }}
+    |- {{ GenRegs (fmg, fmo, fml, fmi) ** Rwim |=> W v ** {| id, fm1 :: fm2 :: F |} ** p }}
         restore rs oexp rd
-      {{ GenRegs (upd_genreg (fmg, fmi, fm1, fm2) rd (v1 +ᵢ v2)) ** Rwim |=> v **
+      {{ GenRegs (upd_genreg (fmg, fmi, fm1, fm2) rd res) ** Rwim |=> W v **
                  {| id', F ++ [fmo; fml] |} ** p }}.
 Proof.
-  intros.
+  introv Hres; intros.
   eapply ins_conseq_rule.
-  instantiate (1 := Rwim |=> v ** GenRegs (fmg, fmo, fml, fmi) **
+  instantiate (1 := Rwim |=> W v ** GenRegs (fmg, fmo, fml, fmi) **
                          {|id, fm1 :: fm2 :: F|} ** p).
   intros.
   sep_cancel1 1 2.
@@ -1397,8 +1393,6 @@ Proof.
   eapply restore_rule; eauto.
   {
     intros.
-    instantiate (2 := v1).
-    instantiate (1 := v2).
     simpl.
     sep_star_split_tac.
     simpl in H6, H7.
@@ -1441,11 +1435,11 @@ Qed.
 
 Theorem subcc_rule_reg :
   forall oexp (rs rd : GenReg) v1 v2 v grst vn vz p,
-    get_genreg_val grst rs = v1 ->
-    eval_opexp_reg grst oexp = Some v2 -> v = v1 -ᵢ v2 ->
+    get_genreg_val grst rs = W v1 ->
+    eval_opexp_reg grst oexp = Some (W v2) -> v = v1 -ᵢ v2 ->
     |- {{ GenRegs grst ** n |=> vn ** z |=> vz ** p  }}
         subcc rs oexp rd
-      {{ GenRegs (upd_genreg grst rd v) ** n |=> get_range 31 31 v ** z |=> iszero v ** p }}.
+      {{ GenRegs (upd_genreg grst rd (W v)) ** n |=> W (get_range 31 31 v) ** z |=> W (iszero v) ** p }}.
 Proof.
   intros.
   eapply ins_conseq_rule.
@@ -1461,8 +1455,8 @@ Proof.
     simpl in H3, H5, H6.
     simpljoin1.
     simpl.
-    eapply get_R_merge_still; eauto.
-    eapply getR_eq_get_genreg_val; eauto.
+    eapply get_R_merge_still; eauto. 
+    eapply getR_eq_get_genreg_val in H4; rewrite H4, H; eauto.
     sep_star_split_tac.
     simpl in H3, H5, H6.
     simpljoin1.
@@ -1493,20 +1487,18 @@ Qed.
 
 Theorem andcc_rule_reg :
   forall oexp (rs rd : GenReg) v1 v2 v grst vn vz p,
-    get_genreg_val grst rs = v1 ->
-    eval_opexp_reg grst oexp = Some v2 -> v = v1 &ᵢ v2 ->
+    get_genreg_val grst rs = W v1 ->
+    eval_opexp_reg grst oexp = Some (W v2) -> v = v1 &ᵢ v2 ->
     |- {{ GenRegs grst ** n |=> vn ** z |=> vz ** p  }}
         andcc rs oexp rd
-      {{ GenRegs (upd_genreg grst rd v) ** n |=> get_range 31 31 v ** z |=> iszero v ** p }}.
+      {{ GenRegs (upd_genreg grst rd (W v)) ** n |=> W (get_range 31 31 v) ** z |=> W (iszero v) ** p }}.
 Proof.
   intros.
   eapply ins_conseq_rule.
   eauto.
-  eapply andcc_rule.
+  eapply andcc_rule; eauto.
   {
     introv Hs.
-    instantiate (2 := v1).
-    instantiate (1 := v2).
     simpl.
     split.
     sep_star_split_tac.
@@ -1514,16 +1506,13 @@ Proof.
     simpljoin1.
     simpl.
     eapply get_R_merge_still; eauto.
-    eapply getR_eq_get_genreg_val; eauto.
+    eapply getR_eq_get_genreg_val in H4; eauto; rewrite H4, H; eauto.
     sep_star_split_tac.
     simpl in H3, H5, H6.
     simpljoin1.
     simpl.
     eapply eval_opexp_merge_still; eauto.
     eapply eval_opexp_reg_eq_eval_opexp; eauto.
-  }
-  {
-    eauto.
   }
   {
     introv Hs.
@@ -1545,13 +1534,13 @@ Qed.
 
 Theorem rd_rule_reg :
   forall (rsp : SpReg) v (rr : GenReg) p grst,
-    |- {{ GenRegs grst ** rsp |=> v ** p }}
+    |- {{ GenRegs grst ** rsp |=> W v ** p }}
         rd rsp rr
-      {{ GenRegs (upd_genreg grst rr v) ** rsp |=> v ** p }}.
+      {{ GenRegs (upd_genreg grst rr (W v)) ** rsp |=> W v ** p }}.
 Proof.
   intros.
   eapply ins_conseq_rule with
-  (p1 := rsp |=> v ** rr |=> get_genreg_val' grst rr ** GenRegs_rm_one grst rr ** p).
+  (p1 := rsp |=> W v ** rr |=> get_genreg_val' grst rr ** GenRegs_rm_one grst rr ** p).
   Focus 2.
   eapply rd_rule; eauto.
   introv Hs.
@@ -1564,8 +1553,8 @@ Qed.
 
 Theorem wr_rule_reg :
   forall oexp (rs : GenReg) v1 v2 v grst (rsp : SpReg) p,
-    get_genreg_val grst rs = v1 ->
-    eval_opexp_reg grst oexp = Some v2 ->
+    get_genreg_val grst rs = W v1 ->
+    eval_opexp_reg grst oexp = Some (W v2) ->
     |- {{ GenRegs grst ** rsp |=> v ** p }}
         wr rs oexp rsp
       {{ GenRegs grst ** 3 @ rsp |==> set_spec_reg rsp (v1 xor v2) ** p }}.
@@ -1581,14 +1570,13 @@ Proof.
   simpl.
   split.
   
-    subst.
+    subst. 
     sep_star_split_tac.
-    simpl in H3, H4.
+    simpl in H4, H5.
     simpljoin1.
     simpl.
     eapply get_R_merge_still; eauto.
-    eapply getR_eq_get_genreg_val; eauto.
-  
+    eapply getR_eq_get_genreg_val in H3; eauto; rewrite H3, H; eauto.  
   
     sep_star_split_tac.
     simpl in H4, H5.
