coqimp/example/spec/spec.v
@@ -37,51 +37,52 @@ Definition winvalid x y :=
 (** Specification *)
 Definition add_pre (vl : list logicvar) :=
   EX x y z w fret,
-  [| vl = logic_lv x :: logic_lv y :: logic_lv z :: logic_lv fret :: nil |] **
-  i0 |=> x ** i1 |=> y ** i2 |=> z ** l7 |=> w ** r15 |=> fret.
+  [| vl = logic_lw x :: logic_lw y :: logic_lw z :: logic_lw fret :: nil |] **
+  i0 |=> W x ** i1 |=> W y ** i2 |=> W z ** l7 |=> w ** r15 |=> W fret.
 
 Definition add_post (vl : list logicvar) :=
   EX x y z fret,
-  [| vl = logic_lv x :: logic_lv y :: logic_lv z :: logic_lv fret :: nil |] **
-  i0 |=> x ** i1 |=> y ** i2 |=> z ** l7 |=> (x +ᵢ y +ᵢ z) ** r15 |=> fret.
+  [| vl = logic_lw x :: logic_lw y :: logic_lw z :: logic_lw fret :: nil |] **
+  i0 |=> W x ** i1 |=> W y ** i2 |=> W z ** l7 |=> W (x +ᵢ y +ᵢ z) ** r15 |=> W fret.
 
 Definition changeY_pre (vl : list logicvar) :=
   EX fmg fmo fml fmi fret x vy vi id fm1 fm2 F,
   [| vl = logic_fm fmg :: logic_fm fmi :: logic_fm fm1 :: logic_fm fm2
-          :: logic_lv x :: logic_lv fret :: logic_lv vy :: logic_lv vi :: logic_fmls F :: nil |] **
-  GenRegs (fmg, fmo, fml, fmi) ** Ry |=> vy ** Rwim |=> vi ** {| id, fm1 :: fm2 :: F |} **
-  [| get_frame_nth fmi 7 = Some fret /\ get_frame_nth fmi 0 = Some x
+          :: logic_lw x :: logic_lw fret :: logic_lw vy :: logic_lw vi :: logic_fmls F :: nil |] **
+  GenRegs (fmg, fmo, fml, fmi) ** Ry |=> W vy ** Rwim |=> W vi ** {| id, fm1 :: fm2 :: F |} **
+  [| get_frame_nth fmi 7 = Some (W fret) /\ get_frame_nth fmi 0 = Some (W x)
      /\ winvalid (post_cwp id) vi /\ $ 0 <=ᵤᵢ id <=ᵤᵢ $ 7 |].
 
 Definition changeY_post (vl : list logicvar) :=
   EX fmg fmo fml fmi fret x vy vi id fm1 fm2 F,
   [| vl = logic_fm fmg :: logic_fm fmi :: logic_fm fm1 :: logic_fm fm2
-          :: logic_lv x :: logic_lv fret :: logic_lv vy :: logic_lv vi :: logic_fmls F :: nil |] **
-  GenRegs (fmg, (update_frame fmi 0 vy), fm1, fm2) ** Ry |=> x ** Rwim |=> vi **
+          :: logic_lw x :: logic_lw fret :: logic_lw vy :: logic_lw vi :: logic_fmls F :: nil |] **
+  GenRegs (fmg, (update_frame fmi 0 (W vy)), fm1, fm2) ** Ry |=> W x ** Rwim |=> W vi **
   {| post_cwp id, F ++ (fmo :: fml :: nil) |}.
 
 Definition sum3_pre1 (vl : list logicvar) :=
-  EX x y z fret fmg fmo fml fmi id vi F fm1 fm2,
-  [| vl = logic_lv x :: logic_lv y :: logic_lv z :: logic_lv fret :: logic_fm fmg :: nil |] **
-  GenRegs (fmg, fmo, fml, fmi) ** Rwim |=> vi ** {| id, F ++ (fm1 :: fm2 :: nil) |} ** 
-  [| get_frame_nth fmo 0 = Some x /\ get_frame_nth fmo 1 = Some y /\
-     get_frame_nth fmo 2 = Some z /\ get_frame_nth fmo 7 = Some fret /\
-     winvalid id vi /\ winvalid (pre_cwp id) vi /\ $ 0 <=ᵤᵢ id <=ᵤᵢ $ 7 |].
+  EX x y z fret fmg fmo fml fmi id vi F fm1 fm2 b o,
+  [| vl = logic_lw x :: logic_lw y :: logic_lw z :: logic_lw fret :: logic_fm fmg :: logic_lv (Ptr (b, o)) :: nil |] **
+  GenRegs (fmg, fmo, fml, fmi) ** Rwim |=> W vi ** {| id, F ++ (fm1 :: fm2 :: nil) |} ** 
+  [| get_frame_nth fmo 0 = Some (W x) /\ get_frame_nth fmo 1 = Some (W y) /\
+     get_frame_nth fmo 2 = Some (W z) /\ get_frame_nth fmo 7 = Some (W fret) /\
+     winvalid id vi /\ winvalid (pre_cwp id) vi /\ $ 0 <=ᵤᵢ id <=ᵤᵢ $ 7
+     /\ get_frame_nth fmo 6 = Some (Ptr (b, o)) |].
 
 Definition sum3_post1 (vl : list logicvar) :=
-  EX x y z fret fmg fmo fml fmi id vi F fm1 fm2,
-  [| vl = logic_lv x :: logic_lv y :: logic_lv z :: logic_lv fret :: logic_fm fmg :: nil |] **
-  GenRegs (fmg, fmo, fml, fmi) ** Rwim |=> vi ** {| id, F ++ (fm1 :: fm2 :: nil) |} **
-  [| get_frame_nth fmo 0 = Some (x +ᵢ y +ᵢ z) /\ get_frame_nth fmo 7 = Some fret /\
+  EX x y z fret fmg fmo fml fmi id vi F fm1 fm2 b o,
+  [| vl = logic_lw x :: logic_lw y :: logic_lw z :: logic_lw fret :: logic_fm fmg :: logic_lv (Ptr (b, o)) :: nil |] **
+  GenRegs (fmg, fmo, fml, fmi) ** Rwim |=> W vi ** {| id, F ++ (fm1 :: fm2 :: nil) |} **
+  [| get_frame_nth fmo 0 = Some (W x +ᵢ y +ᵢ z) /\ get_frame_nth fmo 7 = Some (W fret) /\
      winvalid id vi /\ winvalid (pre_cwp id) vi /\ $ 0 <=ᵤᵢ id <=ᵤᵢ $ 7 |].
 
-Fixpoint convert_spec (ls : list (Address * fspec)) :
+Fixpoint convert_spec (ls : list (Word * fspec)) :
   funspec :=
   match ls with
-  | nil => fun _ : Address => None
+  | nil => fun _ : Word => None
   | (f', spec) :: ls' =>
-    fun f : Address =>
-      if AddrEq.eq f f' then
+    fun f : Word =>
+      if Int.eq_dec f f' then
         Some spec
       else
         convert_spec ls' f
