coqimp/ext/highlang.v
@@ -1,0 +1,292 @@
+(** We define high-level Pseudo-SPARCv8 language in this File *)
+Require Import Coqlib.
+Require Import Maps.
+
+Require Import Integers.
+Require Import LibTactics.
+Open Scope Z_scope.
+Import ListNotations.
+
+Require Import state.
+Require Import language.
+
+(** Command : expanded the original command with Psave w, Prestore, print *)
+Inductive Command :=
+| c : command -> Command
+| Psave : Word -> Command
+| Prestore : Command
+| print : Command. 
+
+(** The high-level msg : tau | out(v) | call(f, list v) *)
+Inductive msg :=
+| tau : msg
+| out : Val -> msg
+| Callevt : Word -> list Val -> msg.
+
+(** The Code heap *)
+Definition XCodeHeap := CodeMap.t (option Command).
+
+(*+ High-level Program State +*)
+
+(*! Thread Id !*)
+Definition Tid := Z.
+
+(*! Thread Local State !*)
+(* High-level RegName *)
+Inductive HRegName :=
+| hRr : GenReg -> HRegName
+| fn : HRegName
+| fz : HRegName.
+
+Coercion hRr : GenReg >-> HRegName.
+
+(* High-level Register File *)
+Lemma HRegName_eq : forall (x y : HRegName),
+    {x = y} + {x <> y}.
+Proof.
+  repeat decide equality.
+Qed.
+
+Module HRegNameEq.
+  Definition t := HRegName.
+  Definition eq := HRegName_eq.
+End HRegNameEq.
+
+Module HRegMap := EMap(HRegNameEq).
+Definition HRegFile := HRegMap.t (option Val).
+Definition HEmpRFile : HRegFile := fun _ => None.
+
+(* High-level Frame list *)
+Definition HFrame : Type := Z * Frame * Frame.
+Definition HFrameList := list HFrame.
+
+(* High-level Rstate *)
+Definition HRstate : Type := HRegFile * Z * HFrameList.
+
+(* Thread local state *)
+Definition tlocst : Type := HRstate * Word * Word.
+
+(*! Thread Pool !*)
+Module TidEq.
+  Definition t := Tid.
+  Definition eq := Z.eq_dec.
+End TidEq.
+
+Module ThrdMap := EMap(TidEq).
+Definition ThrdPool := ThrdMap.t (option tlocst).
+Definition EmpThrdPool : ThrdPool := fun _ => None.
+
+(*! High-level State !*) 
+Definition HState : Type := ThrdPool * Tid * tlocst * Memory.
+
+(*! Abstract Assembly Primitive Set !*)
+Definition ap := list Val -> HState -> HState -> Prop.
+Definition apSet := CodeMap.t (option ap).
+
+(*! High-level Code  !*) 
+Definition HCode : Type := XCodeHeap * apSet.
+
+(*! High-level Program !*)
+Definition HProg : Type := HCode * HState.
+
+(*+ Operational Semantics for High-level Program +*)
+Definition get_HR (HR : HRegFile) (hrn : HRegName) :=
+  match (HR hrn) with
+  | Some v => match hrn with
+             | hRr r0 => Some (W ($ 0))
+             | _ => Some v
+             end
+  | None => None
+  end.
+
+Definition Heval_opexp (HR : HRegFile) (o : OpExp) :=
+  match o with
+  | Or r => get_HR HR (hRr r)
+  | Ow w =>
+    if andb (($-4096) <=ᵢ w) (w <=ᵢ ($4095)) then
+      Some (W w)
+    else
+      None
+  end.
+
+Definition Heval_addrexp (HR : HRegFile) (a : AddrExp) :=
+  match a with
+  | Ao o => Heval_opexp HR o
+  | Aro r o =>
+    match get_HR HR (hRr r) with
+    | Some v1 =>
+      match (Heval_opexp HR o) with
+      | Some v2 => val_add v1 v2
+      | None => None
+      end 
+    | None => None
+    end
+  end.
+
+Definition set_HR :=
+  fun HR hrn (v : Val) => if is_indom hrn HR then HRegMap.set hrn (Some v) HR else HR.
+
+Fixpoint set_HRs HR (vl : list (HRegName * Val)) : HRegFile :=
+  match vl with
+  | [] => HR
+  | (hrr, v) :: vl0 => set_HRs (set_HR HR hrr v) vl0
+  end.
+
+(** Memory fresh *)
+Definition Mfresh (b : Z) (M : Memory) := forall o, ~ indom (b, o) M.
+
+(** Memory alloc *) 
+Definition Malloc (M : Memory) (b : Z) (l h : Word) (M' : Memory) :=
+  Mfresh b M /\
+  (forall b' o', (b <> b' /\ M (b', o') = M' (b', o'))
+            \/ (b = b' /\ if int_le l o' && Int.lt o' h then
+                            (exists v, M' (b', o') = Some v)
+                          else M'(b', o') = M(b', o'))).
+
+(** Memory free *)
+Definition Mfree (M : Memory) (b : Z) (M' : Memory) :=
+  Mfresh b M' /\
+  (forall b' o', b <> b' -> M (b', o') = M' (b', o')).
+
+Definition Hfetch HR :=
+  match fetch_frame HR r8 r9 r10 r11 r12 r13 r14 r15 with
+  | Some fmo =>
+    match fetch_frame HR r16 r17 r18 r19 r20 r21 r22 r23 with
+    | Some fml =>
+      match fetch_frame HR r24 r25 r26 r27 r28 r29 r30 r31 with
+      | Some fmi => Some [fmo; fml; fmi]
+      | None => None
+      end
+    | None => None
+    end
+  | None => None
+  end.
+
+Definition set_Hframe (HR : HRegFile) (rr0 rr1 rr2 rr3 rr4 rr5 rr6 rr7 : GenReg) (fm : Frame) :=
+  match fm with
+  | consfm v0 v1 v2 v3 v4 v5 v6 v7 =>
+    set_HRs HR [(hRr rr0, v0); (hRr rr1, v1);
+                  (hRr rr2, v2); (hRr rr3, v3); (hRr rr4, v4);
+                    (hRr rr5, v5); (hRr rr6, v6); (hRr rr7, v7)]
+  end.
+
+Definition set_Hwindow (HR : HRegFile) (fm1 fm2 fm3 : Frame) :=
+  let HR1 := set_Hframe HR r8 r9 r10 r11 r12 r13 r14 r15 fm1 in
+  let HR2 := set_Hframe HR1 r16 r17 r18 r19 r20 r21 r22 r23 fm2 in
+  set_Hframe HR2 r24 r25 r26 r27 r28 r29 r30 r31 fm3.
+
+Inductive HQ__ : Memory * HRstate -> Command -> Memory * HRstate -> Prop :=
+| HLd_step : forall aexp (ri : GenReg) (M : Memory) HR HR' HF addr v b,
+    Heval_addrexp HR aexp = Some (Ptr addr) ->
+    word_aligned (Ptr addr) = true ->
+    M addr = Some v ->
+    indom ri HR -> set_HR HR ri v = HR' ->
+    HQ__ (M, (HR, b, HF)) (c (cntrans (ld aexp ri))) (M, (HR', b, HF))
+
+| HST_step : forall aexp (ri : GenReg) (M M' : Memory) HR HF addr v b,
+    Heval_addrexp HR aexp = Some (Ptr addr) ->
+    word_aligned (Ptr addr) = true ->
+    get_HR HR ri = Some v ->
+    indom addr M -> MemMap.set addr (Some v) M = M' ->
+    HQ__ (M, (HR, b, HF)) (c (cntrans (st ri aexp))) (M', (HR, b, HF))
+
+| HNop_step : forall M HR b HF,
+    HQ__ (M, (HR, b, HF)) (c (cntrans nop)) (M, (HR, b, HF))
+
+| HAdd_step : forall M HR HR' oexp (rs rd : GenReg) (v1 v2 v : Val) b HF,
+    get_HR HR rs = Some v1 ->
+    Heval_opexp HR oexp = Some v2 ->
+    indom rd HR -> set_HR HR rd v = HR' -> val_add v1 v2 = Some v ->
+    HQ__ (M, (HR, b, HF)) (c (cntrans (add rs oexp rd))) (M, (HR', b, HF))
+
+| HSub_step : forall M HR HR' oexp (rs rd : GenReg) (v1 v2 v : Val) b HF,
+    get_HR HR rs = Some v1 ->
+    Heval_opexp HR oexp = Some v2 ->
+    indom rd HR -> set_HR HR rd v = HR' -> val_sub v1 v2 = Some v ->
+    HQ__ (M, (HR, b, HF)) (c (cntrans (sub rs oexp rd))) (M, (HR', b, HF))
+
+| HSubcc_step : forall M HR HR' oexp (rs rd : GenReg) (v1 v2 v : Word) b HF,
+    get_HR HR rs = Some (W v1) ->
+    Heval_opexp HR oexp = Some (W v2) ->
+    indom rd HR -> indom fn HR -> indom fz HR -> v = v1 -ᵢ v2 ->
+    set_HRs HR [(hRr rd, W v); (fn, W (get_range 31 31 v)); (fz, W (iszero v))] = HR' ->
+    HQ__ (M, (HR, b, HF)) (c (cntrans (subcc rs oexp rd))) (M, (HR', b, HF))
+
+(* We add two Pseudo instructions : Psave and Prestore *)
+| HPsave_step : forall M M' (HR HR' : HRegFile) sz b b' (HF : HFrameList) fmo fml fmi fm1 fm2,
+    Hfetch HR = Some [fmo; fml; fmi] ->
+    HR' = set_Hwindow HR fm1 fm2 fmo ->
+    Malloc M b' ($ 64) sz M' ->
+    HQ__ (M, (HR, b, HF)) (Psave sz) (M', (HR', b', (b, fml, fmi) :: HF))
+
+| HRestore_step : forall M M' (HR HR' : HRegFile) (b b' : Z) (HF : HFrameList) fmo fml fmi fm1 fm2,
+    Hfetch HR = Some [fmo; fml; fmi] ->
+    Mfree M b M' -> HR r14 = Some (Ptr (b', $ 0)) ->
+    HR' = set_Hwindow HR fmi fm1 fm2 ->
+    HQ__ (M, (HR, b, (b', fm1, fm2) :: HF)) Prestore (M', (HR', b', HF)).
+
+Parameter args : HRstate -> Memory -> list Val -> Prop.
+
+Inductive HH__ : XCodeHeap -> tlocst * Memory -> msg -> tlocst * Memory -> Prop :=
+| HNTrans : forall C pc npc HQ HQ' HM HM' c,
+    C pc = Some c -> HQ__ (HM, HQ) c (HM', HQ') ->
+    HH__ C ((HQ, pc, npc), HM) tau ((HQ', npc, npc +ᵢ ($ 4)), HM')
+
+| HJumpl : forall C HM aexp rd HR HR' b HF pc npc f,
+    C pc = Some (c (cjumpl aexp rd)) ->
+    Heval_addrexp HR aexp = Some (W f) ->
+    word_aligned (W f) = true -> indom rd HR -> set_HR HR rd (W pc) = HR' ->
+    HH__ C (((HR, b, HF), pc, npc), HM) tau (((HR', b, HF), npc, f), HM)
+
+| HCall : forall C HM (HR HR' : HRegFile) HF b pc npc f,
+    C pc = Some (c (ccall f)) ->
+    indom r15 HR -> set_HR HR r15 (W pc) = HR' ->
+    HH__ C (((HR, b, HF), pc, npc), HM) tau (((HR', b, HF), npc, f), HM)
+
+| HRetl : forall C HM HR HF pc npc f b,
+    C pc = Some (c cretl) ->
+    get_HR HR r15 = Some (W f) ->
+    HH__ C (((HR, b, HF), pc, npc), HM) tau (((HR, b, HF), npc, f +ᵢ ($ 8)), HM)
+
+| HBe_true : forall C HM HR HF pc npc f v b,
+    C pc = Some (c (cbe f)) ->
+    get_HR HR fz = Some (W v) -> v <> $ 0 ->
+    HH__ C (((HR, b, HF), pc, npc), HM) tau (((HR, b, HF), npc, f), HM)
+
+| HBe_false : forall C HM HR HF pc npc f b,
+    C pc = Some (c (cbe f)) ->
+    get_HR HR fz = Some (W ($ 0)) ->
+    HH__ C (((HR, b, HF), pc, npc), HM) tau (((HR, b, HF), npc, npc +ᵢ ($ 4)), HM)
+
+(* We add two rules : print, occur an output; and occur a call event *)
+| HPrint : forall C HM HR HF pc npc b v,
+    C pc = Some print -> get_HR HR r8 = Some v ->
+    HH__ C (((HR, b, HF), pc, npc), HM) (out v) ((((HR, b, HF), npc, npc +ᵢ ($ 4)), HM))
+
+| HCallEvt : forall C HQ (pc npc : Word) HM lv,
+    ~ indom pc C -> args HQ HM lv ->
+    HH__ C ((HQ, pc, npc), HM) (Callevt pc lv) ((HQ, pc, npc), HM).
+
+Inductive HP__ : HProg -> msg -> HProg -> Prop :=
+| Htau_step : forall C PrimSet T t K K' HM HM',
+    HH__ C (K, HM) tau (K', HM') ->
+    HP__ ((C, PrimSet), (T, t, K, HM)) tau ((C, PrimSet), (T, t, K', HM'))
+
+| He_step : forall C PrimSet T t K K' HM v,
+    HH__ C (K, HM) (out v) (K', HM) ->
+    HP__ ((C, PrimSet), (T, t, K, HM)) (out v) ((C, PrimSet), (T, t, K', HM))
+
+| Hp_step : forall C (PrimSet : apSet) T T' t t' K K' K'' HM HM' f lv prim,
+    HH__ C (K, HM) (Callevt f lv) (K', HM) -> PrimSet f = Some prim ->
+    prim lv (T, t, K', HM) (T', t', K'', HM') ->
+    HP__ ((C, PrimSet), (T, t, K, HM)) tau ((C, PrimSet), (T', t', K'', HM')).
+
+(* star steps *)
+Inductive HP__star_step : HProg -> HProg -> Prop :=
+| zero_step : forall hp, HP__star_step hp hp
+| multi_step : forall hp hp' hp'' m,
+    HP__ hp m hp' -> HP__star_step hp' hp''.
+
+(* High-level Program Safety *)
+Definition HProgSafe (hp : HProg) :=
+  forall hp', HP__star_step hp hp' -> (exists hp'' m,  HP__ hp' m hp'').
